AwsCryptographicMaterialProviders/test/TestUtils.dfy
@@ -13,6 +13,18 @@ module TestUtils {
   import Types = AwsCryptographyMaterialProvidersTypes
   import Materials
 
+  // These are public resources and MUST NOT be used in any production environment
+  const KMS_RSA_PUBLIC_KEY := "-----BEGIN PUBLIC KEY-----\n"
+   + "MIIBIjANBgkqhkiG9w0BAQEFAAOCAQ8AMIIBCgKCAQEA27Uc/fBaMVhxCE/SpCMQ\n"
+   + "oSBRSzQJw+o2hBaA+FiPGtiJ/aPy7sn18aCkelaSj4kwoC79b/arNHlkjc7OJFsN\n"
+   + "/GoFKgNvaiY4lOeJqEiWQGSSgHtsJLdbO2u4OOSxh8qIRAMKbMgQDVX4FR/PLKeK\n"
+   + "fc2aCDvcNSpAM++8NlNmv7+xQBJydr5ce91eISbHkFRkK3/bAM+1iddupoRw4Wo2\n"
+   + "r3avzrg5xBHmzR7u1FTab22Op3Hgb2dBLZH43wNKAceVwKqKA8UNAxashFON7xK9\n"
+   + "yy4kfOL0Z/nhxRKe4jRZ/5v508qIzgzCksYy7Y3QbMejAtiYnr7s5/d5KWw0swou\n"
+   + "twIDAQAB\n"
+   + "-----END PUBLIC KEY-----";
+  const KMS_RSA_PRIVATE_KEY_ARN := "arn:aws:kms:us-west-2:370957321024:key/mrk-63d386cb70614ea59b32ad65c9315297";
+
   const SHARED_TEST_KEY_ARN := "arn:aws:kms:us-west-2:658956600833:key/b3537ef1-d8dc-4780-9f5a-55776cbb2f7f";
 
   const ACCOUNT_IDS := ["658956600833"];
